Document Interface

src/Shallow/Interface.v
@@ -1,11 +1,29 @@
 Require Import Automation.
 
 Require Import ProgLang.Prog.
+Require Import ProgLang.ProgTheorems.
 Require Import ProgLang.Hoare.
 
-Require Import ProgLang.ProgTheorems.
+(* Interfaces are groups of methods with a shared level of abstraction.
 
-Record InterfaceAPI opT State :=
+A complete, usable interface consists of three logical parts:
+- An API, specifying what each operation does (the types implicitly specify what
+  the operations are)
+- An implementation, giving a program for each operation as well as an overall recovery procedure.
+- A refinement proof that shows each operation behaves as the API specifies with
+  atomic behavior on crash after running the recovery procedure. This proof
+  includes giving a refinement to the abstract state used to specify the API.
+ *)
+
+(* An InterfaceAPI takes [opT], a family of types for the operations. Think of
+[opT] as an inductive type where the parameter specifies what the return value
+of the operation should be. This inductive type will be a set of _symbols_ for
+naming the methods of the API.
+
+The type [State] gives the abstract state of the API; the semantics of each
+operation will be defined in terms of how state of this type is manipulated.
+ *)
+Record InterfaceAPI (opT: Type -> Type) (State:Type) :=
   { op_sem: forall T, opT T -> Semantics State T; }.
 
 Definition background_step {opT State} (bg_step: State -> State -> Prop)
@@ -14,6 +32,8 @@ Definition background_step {opT State} (bg_step: State -> State -> Prop)
                  exists state', bg_step state state' /\
                        step op state' v state''; |}.
 
+(* The specification for each operation. Note that after recovery, the abstract
+state is expected to be atomic. *)
 Definition op_spec opT `(api: InterfaceAPI opT State) `(op: opT T) : Specification unit T unit State :=
   fun (_:unit) state =>
     {|
@@ -27,10 +47,18 @@ Definition op_spec opT `(api: InterfaceAPI opT State) `(op: opT T) : Specificati
            exists v, op_sem api op state v state');
     |}.
 
+(* An InterfaceImpl supplies concrete programs for each method defined by [opT],
+as well as a single global recovery procedure. *)
 Record InterfaceImpl opT :=
   { op_impl: forall T, opT T -> prog T;
     recover_impl: prog unit; }.
 
+(* Finally, an Interface ties everything together: the parameter [api] specifies all details of how the implementation behaves, while the fields give an implementation and a refinement proof.
+
+Of note is that in addition to every method being correct ([impl_ok]), the
+recovery procedure should preserve the behavior of [Ret], namely that nothing
+happens (in terms of abstract states) if the system crashes in a quiescent state
+and recovers. This is guaranteed by the [ret_rec_ok] proof. *)
 Record Interface opT State (api: InterfaceAPI opT State) :=
   { interface_impl: InterfaceImpl opT;
     refinement: Refinement State;
@@ -39,12 +67,11 @@ Record Interface opT State (api: InterfaceAPI opT State) :=
                    (op_impl interface_impl _ op)
                    (recover_impl interface_impl)
                    refinement;
-    (* TODO: rec_noop is a poor name, at least for the layer proof; it's really
-       a [Ret_rok] proof, showing [Ret] is correctly recovered (that is, by not
-       doing anything). *)
-    rec_noop_ok:
+    ret_rec_ok:
       rec_noop (recover_impl interface_impl) refinement }.
 
+(* Helper function to get the implementation of a primitive operation from an
+[Interface]. *)
 Definition Prim opT `{api: InterfaceAPI opT State}
            (i:Interface api)
            {T} (op: opT T) : prog T :=
@@ -78,8 +105,6 @@ Proof.
   repeat deex; eauto.
 Qed.
 
-(* weaker version of prim_ok that requires the postcondition imply the recovery
-postcondition *)
 Theorem prim_ok : forall opT `(api: InterfaceAPI opT State)
                     `(i: Interface api)
                     `(op: opT T)
@@ -97,12 +122,13 @@ Proof.
   eauto using prog_rspec_to_rok, prim_spec.
 Qed.
 
+(* Helper to get the recovery procedure from an [Interface]. *)
 Definition irec opT `(api: InterfaceAPI opT State) `(i: Interface api) : prog unit :=
   recover_impl (interface_impl i).
 
-Lemma irec_noop : forall opT `(api: InterfaceAPI opT State) `(i: Interface api),
+Lemma irec_ret_ok : forall opT `(api: InterfaceAPI opT State) `(i: Interface api),
     rec_noop (irec i) (refinement i).
 Proof.
   intros.
-  eapply rec_noop_ok.
+  eapply ret_rec_ok.
 Qed.
